Weidenbach_Book/IsaSAT/Watched_Literals_VMTF.thy
@@ -1497,7 +1497,7 @@ proof -
   let ?ys' = \<open>set ys'\<close>
   have L_xs_ys: \<open>L \<in> ?xs' \<union> ?ys'\<close>
     using abs_vmtf L unfolding vmtf_\<L>\<^sub>a\<^sub>l\<^sub>l_def
-    by (auto simp: in_\<L>\<^sub>a\<^sub>l\<^sub>l_atm_of_in_atms_of)
+    by (auto simp: in_\<L>\<^sub>a\<^sub>l\<^sub>l_atm_of_in_atms_of_iff)
   have dist: \<open>distinct (xs' @ ys')\<close>
     using vmtf_ns_distinct[OF vmtf_ns] by auto
 
@@ -1912,17 +1912,17 @@ proof -
   have no_next_search_all_defined:
     \<open>(ns', m', fst_As', lst_As', None) \<in> vmtf \<A> M \<Longrightarrow> x \<in># \<L>\<^sub>a\<^sub>l\<^sub>l \<A> \<Longrightarrow> defined_lit M x\<close>
     for x ns' m' fst_As' lst_As' remove
-    by (auto simp: vmtf_def vmtf_\<L>\<^sub>a\<^sub>l\<^sub>l_def in_\<L>\<^sub>a\<^sub>l\<^sub>l_atm_of_in_atms_of
+    by (auto simp: vmtf_def vmtf_\<L>\<^sub>a\<^sub>l\<^sub>l_def in_\<L>\<^sub>a\<^sub>l\<^sub>l_atm_of_in_atms_of_iff
         defined_lit_map lits_of_def)
   have next_search_\<L>\<^sub>a\<^sub>l\<^sub>l:
     \<open>(ns', m', fst_As', lst_As', Some y) \<in> vmtf \<A> M \<Longrightarrow> y \<in> atms_of (\<L>\<^sub>a\<^sub>l\<^sub>l \<A>)\<close>
     for ns' m' fst_As' remove y lst_As'
-    by (auto simp: vmtf_def vmtf_\<L>\<^sub>a\<^sub>l\<^sub>l_def in_\<L>\<^sub>a\<^sub>l\<^sub>l_atm_of_in_atms_of
+    by (auto simp: vmtf_def vmtf_\<L>\<^sub>a\<^sub>l\<^sub>l_def in_\<L>\<^sub>a\<^sub>l\<^sub>l_atm_of_in_atms_of_iff
         defined_lit_map lits_of_def)
   have next_search_le_A':
     \<open>(ns', m', fst_As', lst_As', Some y) \<in> vmtf \<A> M \<Longrightarrow> y < length ns'\<close>
     for ns' m' fst_As' remove y lst_As'
-    by (auto simp: vmtf_def vmtf_\<L>\<^sub>a\<^sub>l\<^sub>l_def in_\<L>\<^sub>a\<^sub>l\<^sub>l_atm_of_in_atms_of
+    by (auto simp: vmtf_def vmtf_\<L>\<^sub>a\<^sub>l\<^sub>l_def in_\<L>\<^sub>a\<^sub>l\<^sub>l_atm_of_in_atms_of_iff
         defined_lit_map lits_of_def)
   show ?thesis
     unfolding vmtf_find_next_undef_def
@@ -1930,20 +1930,20 @@ proof -
        WHILEIT_rule[where R=\<open>{(get_next (ns ! the a), a) |a. a \<noteq> None \<and> the a \<in> atms_of (\<L>\<^sub>a\<^sub>l\<^sub>l \<A>)}\<close>])
     subgoal using vmtf by (rule wf_vmtf_get_next)
     subgoal using next_search vmtf by auto
-    subgoal using vmtf by (auto dest!: next_search_\<L>\<^sub>a\<^sub>l\<^sub>l simp: image_image in_\<L>\<^sub>a\<^sub>l\<^sub>l_atm_of_in_atms_of)
+    subgoal using vmtf by (auto dest!: next_search_\<L>\<^sub>a\<^sub>l\<^sub>l simp: image_image in_\<L>\<^sub>a\<^sub>l\<^sub>l_atm_of_in_atms_of_iff)
     subgoal using vmtf by auto
     subgoal using vmtf by auto
     subgoal using vmtf by (auto dest: next_search_le_A')
-    subgoal by (auto simp: image_image in_\<L>\<^sub>a\<^sub>l\<^sub>l_atm_of_in_atms_of)
+    subgoal by (auto simp: image_image in_\<L>\<^sub>a\<^sub>l\<^sub>l_atm_of_in_atms_of_iff)
         (metis next_search_\<L>\<^sub>a\<^sub>l\<^sub>l option.distinct(1) option.sel vmtf_next_search_take_next)
-    subgoal by (auto simp: image_image in_\<L>\<^sub>a\<^sub>l\<^sub>l_atm_of_in_atms_of)
+    subgoal by (auto simp: image_image in_\<L>\<^sub>a\<^sub>l\<^sub>l_atm_of_in_atms_of_iff)
         (metis next_search_\<L>\<^sub>a\<^sub>l\<^sub>l option.distinct(1) option.sel vmtf_next_search_take_next)
     subgoal by (auto dest: no_next_search_all_defined next_search_\<L>\<^sub>a\<^sub>l\<^sub>l)
     subgoal by (auto dest: next_search_le_A')
     subgoal for x1 ns' x2 m' x2a fst_As' next_search' x2c s
       by (auto dest: no_next_search_all_defined next_search_\<L>\<^sub>a\<^sub>l\<^sub>l)
     subgoal by (auto dest: vmtf_next_search_take_next)
-    subgoal by (auto simp: image_image in_\<L>\<^sub>a\<^sub>l\<^sub>l_atm_of_in_atms_of)
+    subgoal by (auto simp: image_image in_\<L>\<^sub>a\<^sub>l\<^sub>l_atm_of_in_atms_of_iff)
     done
 qed
 
@@ -3017,6 +3017,16 @@ lemma vmtf_unset_pre_vmtf:
 
 definition vmtf_heur_fst where
   \<open>vmtf_heur_fst = (\<lambda>(_, _, a, _). a)\<close>
+
+
+subsection \<open>Hash for lists\<close>
+
+definition atms_hash_insert_pre :: \<open>nat \<Rightarrow> nat list \<times> bool list \<Rightarrow> bool\<close> where
+\<open>atms_hash_insert_pre i = (\<lambda>(n, xs). i < length xs \<and> (\<not>xs!i \<longrightarrow> length n < 2 + unat32_max div 2))\<close>
+
+definition atoms_hash_insert :: \<open>nat \<Rightarrow> nat list \<times> bool list \<Rightarrow> (nat list \<times> bool list)\<close> where
+\<open>atoms_hash_insert i  = (\<lambda>(n, xs). if xs ! i then (n, xs) else (n @ [i], xs[i := True]))\<close>
+
 
 subsection \<open>Phase saving\<close>
 
