Weidenbach_Book/IsaSAT/IsaSAT_Inner_Propagation.thy
@@ -482,7 +482,7 @@ proof -
      apply (rule order_trans)
      apply (rule ref_two_step')
      apply (rule vmtf_mark_to_rescore_also_reasons_cl_spec[OF vm valid C bound H])
-     subgoal by (auto simp: isa_vmtf_def conc_fun_RES)
+     subgoal by (auto simp: conc_fun_RES)
      done
   done
 qed
@@ -510,7 +510,7 @@ proof -
     \<forall>C. Propagated (- L) C \<in> set (get_trail_wl T) \<longrightarrow>
     C \<noteq> 0 \<longrightarrow> C \<in># dom_m (get_clauses_wl T) \<and> (\<forall>C\<in>set [C..<C + arena_length (get_clauses_wl_heur S) C]. arena_lit (get_clauses_wl_heur S) C \<in># \<L>\<^sub>a\<^sub>l\<^sub>l (all_atms_st T))\<close>
     subgoal
-      using valid C by (auto simp: arena_lifting in_\<L>\<^sub>a\<^sub>l\<^sub>l_atm_of_in_atms_of atms_of_\<L>\<^sub>a\<^sub>l\<^sub>l_\<A>\<^sub>i\<^sub>n
+      using valid C by (auto simp: arena_lifting in_\<L>\<^sub>a\<^sub>l\<^sub>l_atm_of_in_atms_of_iff atms_of_\<L>\<^sub>a\<^sub>l\<^sub>l_\<A>\<^sub>i\<^sub>n
         all_atms_st_def all_atms_def all_lits_def all_lits_of_mm_union ran_m_def all_lits_of_mm_add_mset image_Un
         atm_of_all_lits_of_m(2)
         dest!: multi_member_split[of C]
@@ -525,7 +525,7 @@ proof -
         using TU list arena_lifting(5)[OF valid, of D \<open>C - D\<close>,symmetric]
         apply (auto simp: twl_list_invs_def dest!: spec[of _ \<open>-L\<close>] spec[of _ \<open>D\<close>])
         using valid
-        apply (auto simp: in_\<L>\<^sub>a\<^sub>l\<^sub>l_atm_of_in_atms_of atms_of_\<L>\<^sub>a\<^sub>l\<^sub>l_\<A>\<^sub>i\<^sub>n
+        apply (auto simp: in_\<L>\<^sub>a\<^sub>l\<^sub>l_atm_of_in_atms_of_iff atms_of_\<L>\<^sub>a\<^sub>l\<^sub>l_\<A>\<^sub>i\<^sub>n
           all_atms_st_def all_atms_def all_lits_def all_lits_of_mm_union ran_m_def all_lits_of_mm_add_mset image_Un
           atm_of_all_lits_of_m(2) arena_lifting
           dest!: multi_member_split[of D] spec[of _ \<open>-L\<close>] spec[of _ \<open>D\<close>]
