Weidenbach_Book/IsaSAT/IsaSAT_Lookup_Conflict.thy
@@ -297,24 +297,24 @@ proof -
     subgoal for x x' x1 x2 x1a x2a x1b x2b x1c x2c x1d x2d x1e x2e
       using valid i literals_are_in_\<L>\<^sub>i\<^sub>n_mm_in_\<L>\<^sub>a\<^sub>l\<^sub>l[of \<A> N i x1] lits
       by (auto simp: option_lookup_clause_rel_def lookup_clause_rel_def
-        in_\<L>\<^sub>a\<^sub>l\<^sub>l_atm_of_in_atms_of arena_lifting ac_simps get_level_get_level_pol[OF M'M, symmetric]
+        in_\<L>\<^sub>a\<^sub>l\<^sub>l_atm_of_in_atms_of_iff arena_lifting ac_simps get_level_get_level_pol[OF M'M, symmetric]
         isa_outlearned_add_outlearned_add[OF M'M] isa_clvls_add_clvls_add[OF M'M] lev_le)
     subgoal for x x' x1 x2 x1a x2a x1b x2b x1c x2c x1d x2d x1e x2e
       using i literals_are_in_\<L>\<^sub>i\<^sub>n_mm_in_\<L>\<^sub>a\<^sub>l\<^sub>l[of \<A> N i x1] lits valid M'M
       using bxs by (auto simp: option_lookup_clause_rel_def lookup_clause_rel_def
-      in_\<L>\<^sub>a\<^sub>l\<^sub>l_atm_of_in_atms_of arena_lifting ac_simps)
+      in_\<L>\<^sub>a\<^sub>l\<^sub>l_atm_of_in_atms_of_iff arena_lifting ac_simps)
     subgoal for x x' x1 x2 x1a x2a x1b x2b x1c x2c x1d x2d x1e x2e
       using valid i literals_are_in_\<L>\<^sub>i\<^sub>n_mm_in_\<L>\<^sub>a\<^sub>l\<^sub>l[of \<A> N i x1] lits
       by (auto simp: option_lookup_clause_rel_def lookup_clause_rel_def
-        in_\<L>\<^sub>a\<^sub>l\<^sub>l_atm_of_in_atms_of arena_lifting ac_simps get_level_get_level_pol[OF M'M]
+        in_\<L>\<^sub>a\<^sub>l\<^sub>l_atm_of_in_atms_of_iff arena_lifting ac_simps get_level_get_level_pol[OF M'M]
         isa_outlearned_add_outlearned_add[OF M'M] isa_clvls_add_clvls_add[OF M'M])
     subgoal for x x' x1 x2 x1a x2a x1b x2b x1c x2c x1d x2d x1e x2e
       using valid i literals_are_in_\<L>\<^sub>i\<^sub>n_mm_in_\<L>\<^sub>a\<^sub>l\<^sub>l[of \<A> N i x1] lits
       by (auto simp: option_lookup_clause_rel_def lookup_clause_rel_def
-        in_\<L>\<^sub>a\<^sub>l\<^sub>l_atm_of_in_atms_of arena_lifting ac_simps get_level_get_level_pol[OF M'M]
+        in_\<L>\<^sub>a\<^sub>l\<^sub>l_atm_of_in_atms_of_iff arena_lifting ac_simps get_level_get_level_pol[OF M'M]
         isa_outlearned_add_outlearned_add[OF M'M] isa_clvls_add_clvls_add[OF M'M])
     subgoal using bxs by (auto simp: option_lookup_clause_rel_def lookup_clause_rel_def
-      in_\<L>\<^sub>a\<^sub>l\<^sub>l_atm_of_in_atms_of get_level_get_level_pol[OF M'M])
+      in_\<L>\<^sub>a\<^sub>l\<^sub>l_atm_of_in_atms_of_iff get_level_get_level_pol[OF M'M])
     done
 qed
 
@@ -505,7 +505,7 @@ proof -
             dest: in_diffD)
       have [simp]: \<open>atm_of (D ! a) < length xs\<close> \<open>D ! a \<in># \<L>\<^sub>a\<^sub>l\<^sub>l \<A>\<close>
         using literals_are_in_\<L>\<^sub>i\<^sub>n_in_\<L>\<^sub>a\<^sub>l\<^sub>l[OF \<open>literals_are_in_\<L>\<^sub>i\<^sub>n \<A> (mset D)\<close> a_le_D] atms_le_xs
-        by (auto simp: in_\<L>\<^sub>a\<^sub>l\<^sub>l_atm_of_in_atms_of)
+        by (auto simp: in_\<L>\<^sub>a\<^sub>l\<^sub>l_atm_of_in_atms_of_iff)
 
       have ocr: \<open>((False, add_to_lookup_conflict (D ! a) (ab, b)), Some (remdups_mset (?C' (Suc a))))
         \<in> option_lookup_clause_rel \<A>\<close>
@@ -526,7 +526,7 @@ proof -
       case if_cond: False
       have atm_D_a_le_xs: \<open>atm_of (D ! a) < length xs\<close> \<open>D ! a \<in># \<L>\<^sub>a\<^sub>l\<^sub>l \<A>\<close>
         using literals_are_in_\<L>\<^sub>i\<^sub>n_in_\<L>\<^sub>a\<^sub>l\<^sub>l[OF \<open>literals_are_in_\<L>\<^sub>i\<^sub>n \<A> (mset D)\<close> a_le_D] atms_le_xs
-        by (auto simp: in_\<L>\<^sub>a\<^sub>l\<^sub>l_atm_of_in_atms_of)
+        by (auto simp: in_\<L>\<^sub>a\<^sub>l\<^sub>l_atm_of_in_atms_of_iff)
       have [simp]: \<open>D ! a \<notin># C - add_mset (- D ! a)
              (add_mset (D ! a)
                (mset (take a D) + uminus `# mset (take a D)))\<close>
@@ -574,7 +574,7 @@ proof -
               dest: in_diffD)
         have [simp]: \<open>atm_of (D ! a) < length xs\<close> \<open>D ! a \<in># \<L>\<^sub>a\<^sub>l\<^sub>l \<A>\<close>
           using literals_are_in_\<L>\<^sub>i\<^sub>n_in_\<L>\<^sub>a\<^sub>l\<^sub>l[OF \<open>literals_are_in_\<L>\<^sub>i\<^sub>n \<A> (mset D)\<close> a_le_D] atms_le_xs
-          by (auto simp: in_\<L>\<^sub>a\<^sub>l\<^sub>l_atm_of_in_atms_of)
+          by (auto simp: in_\<L>\<^sub>a\<^sub>l\<^sub>l_atm_of_in_atms_of_iff)
 
         show ocr: \<open>((False, add_to_lookup_conflict (D ! a) (ab, b)),
           Some (remdups_mset (?C' (Suc a)))) \<in> option_lookup_clause_rel \<A>\<close>
@@ -694,7 +694,7 @@ proof (standard)
     by (auto dest!: multi_member_split)
   then show \<open>L \<in># \<L>\<^sub>a\<^sub>l\<^sub>l \<A>\<close>
     using lits atm_of_notin_atms_of_iff in_all_lits_of_mm_ain_atms_of_iff
-    unfolding literals_are_in_\<L>\<^sub>i\<^sub>n_mm_def in_\<L>\<^sub>a\<^sub>l\<^sub>l_atm_of_in_atms_of
+    unfolding literals_are_in_\<L>\<^sub>i\<^sub>n_mm_def in_\<L>\<^sub>a\<^sub>l\<^sub>l_atm_of_in_atms_of_iff
     by blast
 qed
 
@@ -3345,7 +3345,7 @@ lemma lookup_conflict_remove1:
     using mset_as_position_remove[of c b \<open>atm_of aa\<close>]
     by (cases \<open>aa\<close>)
       (auto simp: lookup_clause_rel_def lookup_conflict_remove1_def lookup_clause_rel_atm_in_iff
-        minus_notin_trivial2 size_remove1_mset_If in_\<L>\<^sub>a\<^sub>l\<^sub>l_atm_of_in_atms_of minus_notin_trivial
+        minus_notin_trivial2 size_remove1_mset_If in_\<L>\<^sub>a\<^sub>l\<^sub>l_atm_of_in_atms_of_iff minus_notin_trivial
         mset_as_position_in_iff_nth)
    done
 
@@ -3839,7 +3839,7 @@ proof -
   have map: \<open>mset_as_position d yb\<close> and le: \<open>\<forall>L\<in>atms_of (\<L>\<^sub>a\<^sub>l\<^sub>l \<A>). L < length d\<close> and [simp]: \<open>\<not>b\<close>
     using assms by (auto simp: option_lookup_clause_rel_def lookup_clause_rel_def)
   have aa_d: \<open>atm_of aa < length d\<close> and uaa_d: \<open>atm_of (-aa) < length d\<close>
-    using le aa by (auto simp: in_\<L>\<^sub>a\<^sub>l\<^sub>l_atm_of_in_atms_of)
+    using le aa by (auto simp: in_\<L>\<^sub>a\<^sub>l\<^sub>l_atm_of_in_atms_of_iff)
   from mset_as_position_in_iff_nth[OF map aa_d]
   have 1: \<open>(aa \<in># yb) = (d ! atm_of aa = Some (is_pos aa))\<close>
     .
